theories/interop/wp_ext_call_laws.v
@@ -1,7 +1,7 @@
 From melocoton.mlanguage Require Import weakestpre.
 From melocoton.interop.wp_prims Require Export
-  alloc alloc_foreign int2val modify readfield read_foreign
-  registerroot unregisterroot val2int write_foreign.
+  alloc alloc_foreign int2val isblock modify readfield read_foreign
+  read_tag registerroot unregisterroot val2int write_foreign.
 
 Section Laws.
 
@@ -25,6 +25,8 @@ Proof using.
   - apply readfield_correct.
   - apply val2int_correct.
   - apply int2val_correct.
+  - apply isblock_correct.
+  - apply read_tag_correct.
   - apply alloc_foreign_correct.
   - apply write_foreign_correct.
   - apply read_foreign_correct.
